<style>
body {
    font-family: "Times New Roman";
}
body :not(.katex, h1, h2, h3, h4) {
    font-size: 14pt;
}
.break {
    break-after: page;
}
</style>

# Part A

- Student ID: 20240614
- Name: Lee Jongwon

## A-1. Probability

### Q1. Jackpot?

let $J\in\set{+j,-j}$ indicates whether the slot machine is jackpot mode or not,  
and $F\in\set{+f,-f}$ indicates whether it lights flash or not.  
Then the problem is calculating $P(J=+j\mid F=+f)$  

$P(J=+j)=0.025$, $P(F=+f\mid J=+j)=0.8$, $P(F=-f\mid J=-j)=0.1$ are given, then,

$1.\;P(J=+j\mid F=+f)=\dfrac{P(F=+f\mid J=+j)P(J=+j)}{P(F=+f)}$  By `Beyes' Rule`

$2.\;P(F=+f)=P(F=+f\mid J=+j)P(J=+j)+P(F=+f\mid J=-j)P(J=-j)$  
By `Marginalization`

$\Rightarrow P(J=+j\mid F=+f)=\dfrac{P(F=+f\mid J=+j)P(J=+j)}{P(F=+f\mid J=+j)P(J=+j)+P(F=+f\mid J=-j)P(J=-j)}$

<span style="margin-right: 168px;"></span>$=\dfrac{0.8\cdot0.025}{0.8\cdot0.025+0.1\cdot(1-0.025)}$

<span style="margin-right: 168px;"></span>$=\dfrac{8}{47}$

$\therefore P(J=+j\mid F=+f)=\dfrac{8}{47}$

<div class="break"></div>

## A-2. Bayes' Net

### Q2

$P(+b\mid-a,+e)=\dfrac{2}{5}$

### Q3

|sample|weight|
|---|---|
|$−a\;−b\;+c\;+d\;+e$|$P(+e\mid+c,+d)=0.4$|
|$−a\;+b\;+c\;-d\;+e$|$P(+e\mid+c,-d)=0.6$|
|$−a\;−b\;-c\;-d\;+e$|$P(+e\mid-c,-d)=0.6$|
|$−a\;−b\;+c\;-d\;+e$|$P(+e\mid+c,-d)=0.6$|
|$−a\;+b\;+c\;+d\;+e$|$P(+e\mid+c,+d)=0.4$|

$\Rightarrow P(+b\mid-a,+e)$

<span style="margin-right: 50px;"></span>$=\dfrac{P(+e\mid+c,-d)+P(+e\mid+c,+d)}{P(+e\mid+c,+d)+P(+e\mid+c,-d)+P(+e\mid-c,-d)+P(+e\mid+c,-d)+P(+e\mid+c,+d)}$

<span style="margin-right: 50px;"></span>$=\dfrac{0.6+0.4}{0.4+0.6+0.6+0.6+0.4}$

<span style="margin-right: 50px;"></span>$=\dfrac{1}{2.6}$

<span style="margin-right: 50px;"></span>$=\dfrac{5}{13}$

$\therefore P(+b\mid-a,+e)=\dfrac{5}{13}$

<div class="break"></div>

### Q4

$P_{total}=P(E\mid C,D,origin)\cdot P(origin)+P(E\mid C,D,new)\cdot P(new)$

<span style="margin-right: 52px;"></span>$=P_{origin}(E\mid C,D)\cdot0.5+P_{new}(E\mid C,D)\cdot0.5$

Based on above equation, the total CPT is:

|$C$|$D$|$E$|$P_{total}(E\mid C,D)$|
|---|---|---|---|
|$+c$|$+d$|$+e$|$0.4\cdot0.5+0.8\cdot0.5=0.6$|
|$+c$|$+d$|$-e$|$0.6\cdot0.5+0.2\cdot0.5=0.4$|
|$+c$|$-d$|$+e$|$0.6\cdot0.5+0.4\cdot0.5=0.5$|
|$+c$|$-d$|$-e$|$0.4\cdot0.5+0.6\cdot0.5=0.5$|
|$-c$|$+d$|$+e$|$0.2\cdot0.5+0.2\cdot0.5=0.2$|
|$-c$|$+d$|$-e$|$0.8\cdot0.5+0.8\cdot0.5=0.8$|
|$-c$|$-d$|$+e$|$0.6\cdot0.5+0.6\cdot0.5=0.6$|
|$-c$|$-d$|$-e$|$0.4\cdot0.5+0.4\cdot0.5=0.4$|

Based on above CPT, the weight of samples are:

|sample|weight|
|---|---|
|$−a\;−b\;+c\;+d\;+e$|$P(+e\mid+c,+d)=0.6$|
|$−a\;+b\;+c\;-d\;+e$|$P(+e\mid+c,-d)=0.5$|
|$−a\;−b\;-c\;-d\;+e$|$P(+e\mid-c,-d)=0.6$|
|$−a\;−b\;+c\;-d\;+e$|$P(+e\mid+c,-d)=0.5$|
|$−a\;+b\;+c\;+d\;+e$|$P(+e\mid+c,+d)=0.6$|


$\therefore P(+b\mid-a,+e)=\dfrac{0.5+0.6}{0.6+0.5+0.6+0.5+0.6}$

<span style="margin-right: 129px;"></span>$=\dfrac{1.1}{2.8}$

<span style="margin-right: 129px;"></span>$=\dfrac{11}{28}$

### Q5

#### Q5-1

$P(+e\mid+c,-d)=0.6$

#### Q5-2

$P(+a\mid-b)=\dfrac{P(-b\mid+a)P(+a)}{P(-b)}$

<span style="margin-right: 87.5px;"></span>$=\dfrac{P(-b\mid+a)P(+a)}{P(-b\mid+a)P(+a)+P(-b\mid-a)P(-a)}$

<span style="margin-right: 87.5px;"></span>$=\dfrac{0.8\cdot0.5}{0.8\cdot0.5+0.5\cdot0.5}$

<span style="margin-right: 87.5px;"></span>$=\dfrac{0.4}{0.65}$

<span style="margin-right: 87.5px;"></span>$=\dfrac{8}{13}$

#### Q5-3

$P(B\mid A,C,D)\propto P(B\mid A)\times P(C\mid B)\times P(D\mid B)$

$\therefore P(+b\mid-a,+c,-d)=\dfrac{P(+b\mid-a)P(+c\mid+b)P(-d\mid+b)}{P(+b\mid-a)P(+c\mid+b)P(-d\mid+b)+P(-b\mid-a)P(+c\mid-b)P(-d\mid-b)}$

<span style="margin-right: 157px;"></span>$=\dfrac{0.5\cdot0.4\cdot0.8}{0.5\cdot0.4\cdot0.8+0.5\cdot0.8\cdot0.8}$

<span style="margin-right: 157px;"></span>$=\dfrac{0.16}{0.16+0.32}$

<span style="margin-right: 157px;"></span>$=\dfrac{0.16}{0.48}$

<span style="margin-right: 157px;"></span>$=\dfrac{1}{3}$